src/Polara/Optimizations/NbE.lean
@@ -7,220 +7,234 @@ open Ty Tm Const0 Const1 ArithOp AddOp MulOp Const2
 ------------------------------------------------------------------------------------------
 
 -- denotation - corresponding host-anguage value
-@[reducible] def Ty.de (Γ : Ty → Type): Ty → Type
-  | nat => Tm Γ nat
-  | flt => Tm Γ flt
-  | lin => Tm Γ lin
-  | idx i => Tm Γ (idx i)
-  | s ×× t => s.de Γ × t.de Γ
-  | s ~> t => s.de Γ → t.de Γ
-  | array n t => Tm Γ (idx n) → t.de Γ
-  | unit => Tm Γ unit
-  | ref _ => Unit -- not supported in term
+@[reducible] private def Ty.de (Γ : Ty → Type): Ty → Type
+| nat => Tm Γ nat
+| flt => Tm Γ flt
+| lin => Tm Γ lin
+| idx i => Tm Γ (idx i)
+| s ×× t => s.de Γ × t.de Γ
+| s ~> t => s.de Γ → t.de Γ
+| array n t => Tm Γ (idx n) → t.de Γ
+| unit => Tm Γ unit
+| list α => Tm Γ (list α)
 
 instance: Inhabited (Ty.de Γ α) :=
   ⟨
     let rec go := λ
-    | .nat => cst0 (litn 0)
-    | .flt => cst0 (litf 0)
-    | .lin => cst0 (litl 0)
-    | .idx _ => cst0 (liti 0)
+    | .nat => tlitn 0
+    | .flt => tlitf 0
+    | .lin => tlitlZ
+    | .idx _ => tliti 0
     | α ×× β => (go α, go β)
     | _ ~> β => λ _ => go β
     | .array _ α => λ _ => go α
-    | .unit => cst0 litu
-    | .ref _ => ()
+    | .unit => tlitu
+    | list _ => tlitlE
     go α
   ⟩
 
 -- schwache starke c(...) Eta gesetz
 mutual
   -- denotation to term
-  def quote {Γ} : {α : Ty} → Ty.de Γ α → Tm Γ α
-    | unit  , e => e
-    | nat   , e => e
-    | flt   , e => e
-    | lin   , e => e
-    | idx _i, e => e
-    | _α ~> _β   , e => abs fun x => quote (e (splice (var x)))
-    | _α ×× _β   , e => cst2 tup (quote e.1) (quote e.2)
-    | array _n _α, e => bld fun x => quote (e (var x))
-    | .ref _α, _ => panic! "ref not supported in denotation"
+  private def quote {Γ} : {α : Ty} → α.de Γ → Tm Γ α
+  | unit  , e => e
+  | nat   , e => e
+  | flt   , e => e
+  | lin   , e => e
+  | idx _i, e => e
+  | _α ~> _β   , e => fun' x => quote (e (splice x))
+  | _α ×× _β   , e => (quote e.1,, quote e.2)
+  | array _n _α, e => for' x => quote (e x)
+  | list _, e => e
   -- term to denotation
-  def splice {Γ} : {α : Ty} → Tm Γ α → Ty.de Γ α
-    | unit  , e => e
-    | nat   , e => e
-    | flt   , e => e
-    | lin   , e => e
-    | idx _i, e => e
-    | _α ~> _β   , e => fun x => splice (cst2 app e (quote x))
-    | _α ×× _β   , e => (splice (cst1 fst e), splice (cst1 snd e))
-    | array _n _α, e => fun x => splice (cst2 get e x)
-    | .ref _α, _ => panic! "ref not supported in denotation"
+  private def splice {Γ} : {α : Ty} → Tm Γ α → Ty.de Γ α
+  | unit  , e => e
+  | nat   , e => e
+  | flt   , e => e
+  | lin   , e => e
+  | idx _i, e => e
+  | _α ~> _β   , e => λ x => splice (e @@ (quote x))
+  | _α ×× _β   , e => (splice e.fst, splice e.snd)
+  | array _n _α, e => fun x => splice (e[[x]])
+  | list _, e => e
 end
 
-def Const0.de : Const0 α → Ty.de Γ α
-  | litn n => cst0 (litn n)
-  | litf f => cst0 (litf f)
-  | litl l => cst0 (litl l)
-  | liti i => cst0 (liti i)
-  | litu => cst0 litu
-  | mkRef => panic! "ref not supported in denotation"
+private def Const0.de : Const0 α → Ty.de Γ α
+| litn n => tlitn n
+| litf f => tlitf f
+| litlZ => tlitlZ
+| liti i => tliti i
+| litu => tlitu
+| litlE => tlitlE
 
-def Const1.de : Const1 β α → Ty.de Γ β → Ty.de Γ α
-  | fst => fun (a , _b) => a
-  | snd => fun (_a,  b) => b
-  | normCdf => fun
-    -- partial evaluation if argument known
-    | cst0 (litf a) => cst0 (litf (Float.normCdf a))
-    | a             => cst1 normCdf a
-  | sqrt => fun
-    | cst0 (litf a) => cst0 (litf (Float.sqrt a))
-    | a             => cst1 sqrt a
-  | exp => fun
-    | cst0 (litf a) => cst0 (litf (Float.exp a))
-    | a             => cst1 exp a
-  | log => fun
-    | cst0 (litf a) => cst0 (litf (Float.log a))
-    | a             => cst1 log a
-  | sumf => fun a => splice (cst1 sumf (quote a))
-  | suml => fun a => splice (cst1 suml (quote a))
-  | i2n => fun a => splice (cst1 i2n (quote a))
-  | n2f => fun a => splice (cst1 n2f (quote a))
-  | refGet => panic! "ref not supported in denotation"
+private def Const1.de : Const1 β α → Ty.de Γ β → Ty.de Γ α
+| fst => fun (a , _b) => a
+| snd => fun (_a,  b) => b
+| normCdf => fun
+  -- partial evaluation if argument known
+  | cst0 (litf a) => cst0 (litf (Float.normCdf a))
+  | a             => cst1 normCdf a
+| sqrt => fun
+  | cst0 (litf a) => cst0 (litf (Float.sqrt a))
+  | a             => cst1 sqrt a
+| exp => fun
+  | cst0 (litf a) => cst0 (litf (Float.exp a))
+  | a             => cst1 exp a
+| log => fun
+  | cst0 (litf a) => cst0 (litf (Float.log a))
+  | a             => cst1 log a
+| sumf => fun a => splice (cst1 sumf (quote a))
+| suml => fun a => splice (cst1 suml (quote a))
+| i2n => fun
+  | cst0 (liti a) => tlitn a
+  | a => splice (cst1 i2n (quote a))
+| n2f => fun
+  | cst0 (litn a) => tlitf a.toFloat
+  | a => splice (cst1 n2f (quote a))
+| arr2list => λ a => splice (quote a).arr2list
 
-def Tm.isZeroF : Tm Γ α → Bool | cst0 (litf f) => f == 0 | _ => false
-def Tm.isOneF  : Tm Γ α → Bool | cst0 (litf f) => f == 1 | _ => false
+private def Tm.isZeroF : Tm Γ α → Bool | cst0 (litf f) => f == 0 | _ => false
+private def Tm.isOneF  : Tm Γ α → Bool | cst0 (litf f) => f == 1 | _ => false
 
-def Tm.isZeroL : Tm Γ α → Bool | cst0 (litl f) => f == 0 | _ => false
-def Tm.isOneL : Tm Γ α → Bool | cst0 (litl f) => f == 1 | _ => false
+private def arithOpDe (op: ArithOp): BiArrays BiArith α' β' γ'
+→ Ty.de Γ α' → Ty.de Γ β' → Ty.de Γ γ'
+| .array n type =>
+  (λ a b i => arithOpDe op type (a i) (b i))
+| .base t => match t with
+  | .nats =>
+    match op with
+    | .add => fun
+      | .err, _ | _, .err => err
+      | cst0 (litn a), cst0 (litn b) => cst0 (litn (a + b))
+      | cst0 (litn 0), c
+      | c, cst0 (litn 0) => c
+      | a, b => cst2 (arithOp add) a b
+    | .sub => fun
+      | .err, _ | _, .err => err
+      | cst0 (litn a), cst0 (litn b) => cst0 (litn (a - b))
+      | c, cst0 (litn 0) => c
+      | a, b => cst2 (arithOp sub) a b
+    | .mul => fun
+      | .err, _ | _, .err => err
+      | cst0 (litn a), cst0 (litn b) => cst0 (litn (a * b))
+      | a, b => cst2 (arithOp mul) a b
+    | .div => fun
+      | .err, _ | _, .err => err
+      | cst0 (litn a), cst0 (litn b) => if b == 0 then err else cst0 (litn (a / b))
+      | a, b => cst2 (arithOp div) a b
+  | .flts =>
+    match op with
+    | .add => fun
+      | .err, _ | _, .err => err
+      | cst0 (litf a), cst0 (litf b) => cst0 (litf (a + b))
+      | a, b =>
+        if a.isZeroF then b else if b.isZeroF then a else
+        cst2 (arithOp add) a b
+    | .sub => fun
+      | .err, _ | _, .err => err
+      | cst0 (litf a), cst0 (litf b) => cst0 (litf (a - b))
+      | a, b =>
+        if b.isZeroF then a else
+        cst2 (arithOp sub) a b
+    | .mul => fun
+      | .err, _ | _, .err => err
+      | cst0 (litf a), cst0 (litf b) => cst0 (litf (a * b))
+      | a, b =>
+        if      a.isZeroF || b.isZeroF then cst0 (litf 0)
+        else if a.isOneF then b else if b.isOneF then a
+        else cst2 (arithOp mul) a b
+    | .div => fun
+      | .err, _ | _, .err => err
+      | cst0 (litf a), cst0 (litf b) =>
+        if b == 0 then err else cst0 (litf (a / b))
+      | a, b => cst2 (arithOp div) a b
+private def linOpDe (op: AddOp): BiArrays BiLin α' β' γ' → Ty.de Γ α' → Ty.de Γ β' → Ty.de Γ γ'
+| .array n type =>
+  (λ a b i => linOpDe op type (a i) (b i))
+| .base t => match t with
+  | .lins =>
+    match op with
+    | .add => fun
+      | .err, _ | _, .err => err
+      | cst0 litlZ, a | a, cst0 litlZ => a
+      | a, b => a + b
+    | .sub => fun
+      | .err, _ | _, .err => err
+      | a, cst0 litlZ => a
+      | a, b => a - b
+private def linScaleDe (op: MulOp) : BiLF α' β' γ' → Ty.de Γ α' → Ty.de Γ β' → Ty.de Γ γ'
+| .lf => match op with
+  | .mul => fun
+    | .err, _ | _, .err => err
+    | cst0 litlZ, _ => tlitlZ
+    | a, b =>
+      if b.isZeroF then tlitlZ
+      else if b.isOneF then a
+      else a * b
+  | .div => fun
+    | .err, _ | _, .err => err
+    | cst0 litlZ, _ => tlitlZ
+    | a, b =>
+      if b.isZeroF then err
+      else if b.isOneF then a
+      else a / b
 
-def Const2.de : Const2 α β γ → Ty.de Γ α → Ty.de Γ β → Ty.de Γ γ
-  | app => fun f e => f e
-  | get => fun f n => f n
-  | tup => fun a b => (a, b)
-  | lt => fun
-    | .err, _
-    | _, .err => err
-    | cst0 (litf a), cst0 (litf b) => cst0 (litn (if a<b then 1 else 0))
-    | a, b                         => cst2 lt a b
-  | maxf => fun
-    | .err, _ => err
-    | _, .err => err
-    | cst0 (litf a), cst0 (litf b) => cst0 (litf (max a b))
-    | a, b                         => cst2 maxf a b
-  | addi => fun
-    | .err, _
-    | _, err => err
-    -- | cst0 (liti a), cst0 (liti b) => tliti (a.add' b)
-    | a, b => cst2 addi a b
-  | eqi => fun
-    | .err, _
-    | _, err => err
-    | cst0 (liti a), cst0 (liti b) => if a==b then tlitn 1 else tlitn 0
-    | a, b => cst2 eqi a b
-  | @arithOp _ _ _ type op =>
-    let rec goA {α' β' γ': Ty}: BiArrays BiArith α' β' γ' → Ty.de Γ α' → Ty.de Γ β' → Ty.de Γ γ' :=
-      (λ
-        | .array n type =>
-          (λ a b i => goA type (a i) (b i))
-        | .base t => match t with
-          | .nats =>
-            match op with
-            | .add => fun
-              | .err, _ | _, .err => err
-              | cst0 (litn a), cst0 (litn b) => cst0 (litn (a + b))
-              | cst0 (litn 0), c
-              | c, cst0 (litn 0) => c
-              | a, b => cst2 (arithOp add) a b
-            | .sub => fun
-              | .err, _ | _, .err => err
-              | cst0 (litn a), cst0 (litn b) => cst0 (litn (a - b))
-              | c, cst0 (litn 0) => c
-              | a, b => cst2 (arithOp sub) a b
-            | .mul => fun
-              | .err, _ | _, .err => err
-              | cst0 (litn a), cst0 (litn b) => cst0 (litn (a * b))
-              | a, b => cst2 (arithOp mul) a b
-            | .div => fun
-              | .err, _ | _, .err => err
-              | cst0 (litn a), cst0 (litn b) => if b == 0 then err else cst0 (litn (a / b))
-              | a, b => cst2 (arithOp div) a b
-          | .flts =>
-            match op with
-            | .add => fun
-              | .err, _ | _, .err => err
-              | cst0 (litf a), cst0 (litf b) => cst0 (litf (a + b))
-              | a, b =>
-                if a.isZeroF then b else if b.isZeroF then a else
-                cst2 (arithOp add) a b
-            | .sub => fun
-              | .err, _ | _, .err => err
-              | cst0 (litf a), cst0 (litf b) => cst0 (litf (a - b))
-              | a, b =>
-                if b.isZeroF then a else
-                cst2 (arithOp sub) a b
-            | .mul => fun
-              | .err, _ | _, .err => err
-              | cst0 (litf a), cst0 (litf b) => cst0 (litf (a * b))
-              | a, b =>
-                if      a.isZeroF || b.isZeroF then cst0 (litf 0)
-                else if a.isOneF then b else if b.isOneF then a
-                else cst2 (arithOp mul) a b
-            | .div => fun
-              | .err, _ | _, .err => err
-              | cst0 (litf a), cst0 (litf b) =>
-                if b == 0 then err else cst0 (litf (a / b))
-              | a, b => cst2 (arithOp div) a b
-      )
-    goA type.t
-  | @linOp _ _ _ type op =>
-    let rec goL {α' β' γ': Ty}: BiArrays BiLin α' β' γ' → Ty.de Γ α' → Ty.de Γ β' → Ty.de Γ γ' :=
-      (λ
-        | .array n type =>
-          (λ a b i => goL type (a i) (b i))
-        | .base t => match t with
-          | .lins =>
-            match op with
-            | .add => fun
-              | .err, _ | _, .err => err
-              | cst0 (litl a), cst0 (litl b) => cst0 (litl (a + b))
-              | a, b =>
-                if a.isZeroL then b else if b.isZeroL then a else
-                cst2 (linOp add) a b
-            | .sub => fun
-              | .err, _ | _, .err => err
-              | cst0 (litl a), cst0 (litl b) => cst0 (litl (a - b))
-              | a, b =>
-                if b.isZeroL then a else
-                cst2 (linOp sub) a b
-      )
-    goL type.t
-  | @linScale _ _ _ type op =>
-    let rec goS {α' β' γ': Ty}: BiLF α' β' γ' → Ty.de Γ α' → Ty.de Γ β' → Ty.de Γ γ' :=
-      (λ
-        | .lf => match op with
-          | .mul => fun
-            | .err, _ | _, .err => err
-            | cst0 (litl a), cst0 (litf b) => cst0 (litl (a * b))
-            | a, b =>
-              if      a.isZeroL || b.isZeroL then cst0 (litl 0)
-              else if b.isOneL then a
-              else cst2 (linScale mul) a b
-          | .div => fun
-            | .err, _ | _, .err => err
-            | cst0 (litl a), cst0 (litf b) =>
-              if b == 0 then err else cst0 (litl (a / b))
-            | a, b => cst2 (linScale div) a b
-      )
-    match type.t with
-    | .array n t =>
-      (λ a b i => goS t (a i) (b i))
-    | .base t => goS t
-  | refSet => panic! "ref not supported in denotation"
+private def Const2.de : Const2 α β γ → Ty.de Γ α → Ty.de Γ β → Ty.de Γ γ
+| app => fun f e => f e
+| get => fun f n => f n
+| tup => fun a b => (a, b)
+| lt => fun
+  | .err, _
+  | _, .err => err
+  | cst0 (litf a), cst0 (litf b) => cst0 (litn (if a<b then 1 else 0))
+  | a, b                         => cst2 lt a b
+| maxf => fun
+  | .err, _ => err
+  | _, .err => err
+  | cst0 (litf a), cst0 (litf b) => cst0 (litf (max a b))
+  | a, b                         => cst2 maxf a b
+| addi => fun
+  | .err, _
+  | _, err => err
+  | cst0 (liti a (n:=n)), cst0 (liti b (n:=m)) =>
+      tliti (Pos.addMinOne_eq_add_min_one▸a.add' b)
+  | a, b => cst2 addi a b
+| eqi => fun
+  | .err, _
+  | _, err => err
+  | cst0 (liti a), cst0 (liti b) => if a==b then tlitn 1 else tlitn 0
+  | a, b => cst2 eqi a b
+| @arithOp _ _ _ type op => arithOpDe op type.t
+| @linOp _ _ _ type op =>
+  linOpDe op type.t
+| @linScale _ _ _ type op =>
+  match type.t with
+  | .array n t =>
+    (λ a b i => linScaleDe op t (a i) (b i))
+  | .base t => linScaleDe op t
+| @cons _ => λ
+  | e, l => (quote e).cons l
+| @append _ => λ
+  | .err, _ | _, .err => err
+  | cst0 litlE, a | a, cst0 litlE => a
+  | a, b => a.append b
+| @zipL _ _ => λ
+  | .err, _ | _, .err => err
+  | cst0 litlE, _ | _, cst0 litlE => tlitlE
+  | a, b => a.zip b
+| @mapL _ _ => λ
+  | .err, _ => err
+  | cst0 litlE, _ => tlitlE
+  | a, b => a.map (quote b)
+| @aFoldL _ => λ
+  | .err, _ => splice .err
+  | cst0 litlE, (_,n) => n
+  | l, (f, n) => splice (l.aFoldL (quote f) (quote n))
+| @aFoldA _ _ => λ
+  | arr, (f, n) => splice ((quote arr).aFoldA (quote f) (quote n))
 
 -- term in dessen env sich bereich denotierte terme befinden, im prinzip interpreter
-def Tm.de : Tm (Ty.de Γ) α → Ty.de Γ α
+private def Tm.de : Tm (Ty.de Γ) α → Ty.de Γ α
   | var i => i
   | err => splice err
   | cst0 k => k.de
@@ -234,7 +248,7 @@ def Tm.de : Tm (Ty.de Γ) α → Ty.de Γ α
     | cst0 (litn _) => e₂.de
     | a'            => splice (ite a' (quote e₂.de) (quote e₃.de))
 
--- def Tm.safeDe : Tm (Ty.de Γ) α → Ty.de Γ α
+-- private def Tm.safeDe : Tm (Ty.de Γ) α → Ty.de Γ α
 --   | var i => i
 --   | err => splice err
 --   | cst0 k => k.de
