src/Polara/Tests/Examples/All.lean
@@ -1,3 +1,4 @@
 import Polara.Tests.Examples.MultilayerPerceptron
 import Polara.Tests.Examples.PaperCompilingWithArrays
 -- import Polara.Tests.Examples.Thesis
+
