src/Polara/Utils/All.lean
@@ -10,4 +10,5 @@ import Polara.Utils.Utils
 import Polara.Utils.Sigma
 import Polara.Utils.Tests
 import Polara.Utils.Time
+import Polara.Utils.Pos
 
