src/Polara/Utils/Pos.lean
@@ -1,0 +1,32 @@
+structure Pos where
+  val: Nat
+  pos: val≠0
+deriving DecidableEq, Hashable, Repr
+def Nat.toPos (n: Nat)[pos: NeZero n]: Pos := ⟨n,pos.ne⟩
+namespace Pos
+  def toNat := Pos.val
+  theorem zero_lt (p: Pos): 0<p.val := by
+    rw[←@Nat.ne_zero_iff_zero_lt p.val]
+    exact p.pos
+  theorem one_le (p: Pos): 1≤p.val := by
+    have a := zero_lt p
+    have b := @Nat.lt_iff_add_one_le 0 p.val
+    rw [Nat.zero_add] at b
+    rw [b] at a
+    exact a
+  instance instInhabited: Inhabited Pos := ⟨⟨1,by simp⟩⟩
+  instance instNeZero {n: Pos}: NeZero n.toNat := ⟨n.pos⟩
+  instance instCoeNat: Coe Pos Nat := ⟨Pos.toNat⟩
+  instance instOfNat [pos: NeZero n]: OfNat Pos n := ⟨n.toPos⟩
+  instance instToString: ToString Pos := ⟨λ n => ToString.toString n.toNat⟩
+
+  instance instAdd: Add Pos := ⟨λ ⟨a,ap⟩ ⟨b,bp⟩ => ⟨a+b, by simp[ap,bp]⟩⟩
+  def addMinOne: Pos → Pos → Pos := λ ⟨a,ap⟩ ⟨b,bp⟩ => ⟨a-1+b, by simp[ap,bp]⟩
+  theorem addMinOne_eq_add_min_one: (Pos.addMinOne n m).toNat = n.toNat+m.toNat-1 := by
+    let a := (@Nat.sub_add_comm n m 1) (one_le n)
+    simp[Pos.toNat, addMinOne]
+    simp[Pos.toNat] at a
+    rw[a]
+  def finZero(n: Pos): Fin n := ⟨0,n.zero_lt⟩
+  instance instFinOfNat {n: Pos}: OfNat (Fin n) i := ⟨Fin.ofNat' n i⟩
+end Pos
